$$
\begin{align}
\text{Cov}(X,Y)&=\mathbf{E}[(X-\mathbf{E}(X))(Y-\mathbf{E}(Y))]\\
&=\mathbf{E}[XY-X\mathbf{E}(Y)-Y\mathbf{E}(X)+E(X)E(Y)]\\
&=E(XY)-E(X)E(Y)
\end{align}
$$
两个方差非零的随机变量 X 和 Y 的相关系数定义如下：
$$\rho(X,Y)=\frac{\text{cov}(X,Y)}{\sqrt{\text{var}(X)\text{var}(Y)}}$$
当且仅当存在一个正的(负的)常数 c, 使得
$$
Y-\mathrm{E}[Y]=c(X-\mathrm{E}[X])
$$
此时 $\rho=1(-1)$ 
$$
\begin{align}
\mathrm{var}(X_1+X_2)&=E((X_{1}+X_{2}-\mu)^{2})\\
&=E(X_{1}(X_{1}+X_{2}-\mu)+X_{2}(X_{1}+X_{2}-\mu)-\mu(X_{1}+X_{2}-\mu))\\
&=E(X_{1}^2+X_{2}^2+\mu^{2}+2X_{1}X_{2}-2\mu(X_{1}+X_{2}))\\
&=E(X_{1}^{2})+E(X_{2}^{2})+2E(X_{1}X_{2})+\mu^{2}-2\mu^{2}\\
&=E(X_{1}^{2})+E(X_{2}^{2})+2E(X_{1}X_{2})-(\mu_1+\mu_{2})^{2}\\
&=E(X_{1}^{2})-\mu_{1}^2+E(X_{2}^{2})-\mu^{2}+2E(X_{1}X_{2})-2\mu_{1}\mu_{2}\\
&=\mathrm{var}(X_1)+\mathrm{var}(X_2)+2\mathrm{cov}(X_1,X_2),
\end{align}
$$
更一般的结论是
$$\operatorname{var}\left(\sum_{i=1}^nX_i\right)=\sum_{i=1}^n\operatorname{var}(X_i)+\sum_{\{(i,j)|i\neq j\}}\operatorname{cov}(X_i,X_j).$$
![[Pasted image 20240904234507.png]]
![[Pasted image 20240904234609.png]]